src/temporal_logic/feasibility.lean
@@ -1,0 +1,155 @@
+
+import .refinement.one_to_one
+
+universe variables u u₀ u₁ u₂
+
+namespace temporal
+namespace feasibility
+section feasibility
+open fairness predicate nat
+
+parameters {α : Type u}
+parameters {evt : Type u₂}
+parameters {p : pred' α}
+parameters (A : evt → act α)
+parameters {cs₀ fs₀ : evt → pred' α}
+parameters (J : pred' α)
+parameters [inhabited evt] [inhabited α]
+
+parameter init_FIS : ∃ s, s ⊨ p
+parameter init_INV : ∀ s, s ⊨ p → s ⊨ J
+
+parameter evt_FIS : ∀ e s, s ⊨ J → ∃ s', A e s s'
+parameter evt_INV : ∀ e s s', A e s s' → s ⊨ J → s' ⊨ J
+
+def SPEC₀.saf (v : tvar α) : cpred :=
+p ! v ⋀
+◻(∃∃ i, ⟦ v | A i ⟧)
+
+def SPEC₀ (v : tvar α) : cpred :=
+SPEC₀.saf v ⋀
+∀∀ i, sched (cs₀ i ! v) (fs₀ i ! v) ⟦ v | A i ⟧
+
+def p' : pred' (unit × α) :=
+p ! pair.snd
+
+def q' : pred' (unit × unit) :=
+True
+
+def A' (e : evt) : act (unit × α) :=
+A e on prod.snd
+
+def C (e : evt) : act (unit × unit) :=
+λ _ _, true
+
+def C' (e : evt) : act (evt × unit × unit) :=
+λ ⟨sch,_⟩ _, sch = e
+
+abbreviation J' : pred' (unit × α × unit) :=
+J ! pair.fst ! pair.snd
+
+abbreviation cs₀' (e : evt) : pred' (unit × α) :=
+cs₀ e ! pair.snd
+
+abbreviation fs₀' (e : evt) : pred' (unit × α) :=
+fs₀ e ! pair.snd
+
+abbreviation cs₁ (e : evt) : pred' (unit × unit) :=
+True
+
+abbreviation fs₁ (e : evt) : pred' (unit × unit) :=
+True
+section
+include init_FIS init_INV
+lemma SIM₀' (v o : unit)
+  (h : (o, v) ⊨ q')
+: (∃ (w : α), (o, w) ⊨ p' ∧ (o, w, v) ⊨ J') :=
+by { simp [q',p'] at *,
+     apply exists_imp_exists _ init_FIS,
+     intros, split, auto,
+     apply init_INV, assumption }
+end
+open function
+section
+include evt_FIS evt_INV
+lemma SIM' (w : α) (v o v' o' : unit) (e : evt)
+  (hJ : (o, w, v) ⊨ J')
+  (hC : C e (o, v) (o', v'))
+: (∃ (w' : α), A' e (o, w) (o', w') ∧ (o', w', v') ⊨ J') :=
+begin
+  simp [comp,A',on_fun] at *,
+  apply exists_imp_exists _ (evt_FIS e w hJ),
+  tauto,
+end
+
+end
+
+def o : tvar unit := ↑()
+
+-- parameter Hpo
+-- : ∀ c a e, one_to_one_po' (SPEC₀.saf a o ⋀ ◻(J ! ⦃o,a,c⦄))
+--          ⟨cs₁ e,fs₁ e,C' e⟩
+--          ⟨cs₀ e,fs₀ e,A' e⟩ ⦃o,c⦄ ⦃o,a⦄)
+
+
+def SPEC₀.saf' (v : tvar α) (sch : tvar evt) : cpred :=
+p' ! ⦃o,v⦄ ⋀
+◻(∃∃ i, sch ≃ ↑i ⋀ ⟦ o,v | A' i ⟧)
+
+def SPEC₁ (v : tvar unit) : cpred :=
+q' ! ⦃o,v⦄ ⋀
+◻(∃∃ i, ⟦ o,v | C i ⟧) ⋀
+∀∀ i, sched (cs₁ i ! ⦃o,v⦄) (fs₁ i ! ⦃o,v⦄) ⟦ o,v | C i ⟧
+
+lemma Hpo'
+ : ∀ c a e sch, one_to_one_po' (SPEC₁ c ⋀ SPEC₀.saf' a sch ⋀ ◻(J' ! ⦃o,a,c⦄))
+         ⟨cs₁ e!pair.snd,fs₁ e!pair.snd,one_to_one.C' C e⟩
+         ⟨cs₀' e,fs₀' e,A' e⟩ ⦃sch,o,c⦄ ⦃o,a⦄ :=
+begin
+  intros,
+  constructor,
+  { simp [tl_leads_to], },
+  { simp [tl_leads_to], },
+  { simp [tl_leads_to], },
+  begin [temporal]
+    simp [C',SPEC₁,sched,q',action_on _ _ prod.snd,SPEC₀.saf'],
+    intros _ _ _ h _, revert h,
+    monotonicity only,
+    simp, intro,
+    explicit' [C,one_to_one.C',A']
+    { cc, },
+  end
+end
+
+include J init_INV init_FIS evt_INV evt_FIS Hpo'
+lemma feasibility
+: ⊩ (∃∃ v, SPEC₀ v) :=
+begin [temporal]
+  have :=  @one_to_one.refinement α unit unit evt
+     temporal.feasibility.p' temporal.feasibility.q'
+       temporal.feasibility.A'
+       temporal.feasibility.C
+       temporal.feasibility.cs₀'
+       temporal.feasibility.fs₀'
+       temporal.feasibility.cs₁
+       temporal.feasibility.fs₁
+       temporal.feasibility.J' _ _
+       temporal.feasibility.SIM₀'
+       temporal.feasibility.SIM'
+       o _ Γ _,
+  { simp [one_to_one.SPEC₀,SPEC₀] at this ⊢,
+    casesm* [p_exists _, _ ⋀ _],
+    existsi _, auto,
+    split,
+    { simp [SPEC₀.saf,one_to_one.SPEC₀.saf,A',p',action_on' _ _ prod.snd] at *,
+      assumption, },
+    { simp [A',action_on' _ _ prod.snd] at *,
+      assumption, }, },
+  apply temporal.feasibility.Hpo' ,
+  { existsi o,
+    simp [one_to_one.SPEC₁,q',C,C',sched], }
+end
+
+end feasibility
+end feasibility
+end temporal
